Lib/DLList.v
@@ -1,0 +1,311 @@
+From SLFun Require Import Util Values SL VProg.Main.
+
+Import Util.List.
+Import ListNotations SLNotations VProg.Main.Notations FunProg.Notations.
+Import SL.Tactics.
+
+(* Doubly linked lists *)
+
+Module Param.
+  Local Set Implicit Arguments.
+
+  Record lcell_t (D : Type) : Type := mk_lcell {
+    data : D;
+    prev : ptr;
+    next : ptr;
+  }.
+
+  Definition set_prev [D] (prev : ptr) (c : lcell_t D) : lcell_t D :=
+    {| data := data c; prev := prev; next := next c |}.
+
+  Definition set_next [D] (next : ptr) (c : lcell_t D) : lcell_t D :=
+    {| data := data c; prev := prev c; next := next |}.
+
+  Record vp : Type := {
+    data_t : ptr -> Type;
+    vcell  : forall p : ptr, Vprop.p (lcell_t (data_t p));
+    vcell_non_null : forall p v,
+      SLprop.impp (@vcell p v) (p <> NULL)
+  }.
+
+  Definition sel_t (vP : vp) (p : ptr) : Type := lcell_t (data_t vP p).
+
+  Section Fragments.
+    Variable vP : vp.
+
+    Definition read_ref_spec (get : forall p : ptr, sel_t vP p -> ptr) : FDecl SPEC
+      (p : ptr) 'c [vcell vP p ~> c] [] True
+      '(r : ptr) tt [] (r = get p c).
+    Proof. Derived. Defined.
+
+    Definition write_ref_spec (set : forall p : ptr, ptr -> sel_t vP p -> sel_t vP p) : FDecl SPEC
+      ((p, r) : ptr * ptr) 'c [] [vcell vP p ~> c] True
+      '(_ : unit) tt [vcell vP p ~> set p r c] True.
+    Proof. Derived. Defined.
+
+    Record impl (CT : ConcreteProg.context) : Type := {
+      read_prev  : Frag (read_ref_spec  (fun p => @prev _)) CT;
+      write_prev : Frag (write_ref_spec (fun p => @set_prev _)) CT;
+      read_next  : Frag (read_ref_spec  (fun p => @next _)) CT;
+      write_next : Frag (write_ref_spec (fun p => @set_next _)) CT;
+    }.
+  End Fragments.
+End Param.
+
+Section DLList.
+  Import Param.
+  Variable vP : Param.vp.
+
+Section Definitions.
+  (* Doubly linked list segment:
+
+                 first                    last
+           ----> ,---, ----> ,---, ----> ,---, ---->
+      prev       |   |       |   |       |   |       next
+           <---- '---' <---- '---' <---- '---' <----
+
+     NOTE: for an empty segment, [last = prev] and [first = next]
+   *)
+
+  Definition lseg_t := list {p : ptr & data_t vP p}.
+
+
+  Definition lseg_first (l : lseg_t) (sg_next : ptr) : ptr :=
+    match l with
+    | nil               => sg_next
+    | existT _ p _ :: _ => p
+    end.
+
+  Fixpoint lseg_last (sg_prev : ptr) (l : lseg_t) {struct l} : ptr :=
+    match l with
+    | nil               => sg_prev
+    | existT _ p _ :: l => lseg_last p l
+    end.
+
+  Fixpoint lseg_sl (sg_prev : ptr) (l : lseg_t) (sg_next : ptr) {struct l} : SLprop.t :=
+    match l with
+    | nil =>
+        SLprop.emp
+    | (existT _ p d) :: l =>
+        vcell vP p {| data := d; prev := sg_prev; next := lseg_first l sg_next |} **
+        lseg_sl p l sg_next
+    end.
+
+  Definition lseg (prev first next : ptr) (l : lseg_t) : SLprop.t :=
+    SLprop.pure (lseg_first l next = first) **
+    lseg_sl prev l next.
+
+  Definition llist (p : ptr) : Vprop.p lseg_t :=
+    lseg NULL p NULL.
+  Global Arguments llist/.
+End Definitions.
+
+Section Lemmas.
+
+  Derive intro_lseg_nil_spec SuchThat (
+    VLem SPEC ((prev, next) : ptr * ptr)
+    'tt [] [] True
+    '(_ : unit) tt [lseg prev next next ~> nil] True
+    intro_lseg_nil_spec) As intro_lseg_nil.
+  Proof.
+    init_lemma (prev, next) [] ?; unfold lseg; SL.normalize.
+    Apply. auto.
+    reflexivity.
+  Qed.
+
+  Lemma lseg_nil_intro_rule prev next sl :
+    CTX.Trf.Tac.intro_rule true
+      (lseg prev next next ~> sl) []
+      (sl = []) True.
+  Proof.
+    constructor; intros ->; cbn.
+    unfold lseg; SL.normalize.
+    erewrite SLprop.impp_eq. { SL.normalize; reflexivity. }
+    apply SLprop.impp_drop; auto.
+  Qed.
+
+  Derive elim_lseg_nil_spec SuchThat (
+    VLem SPEC ((prev, first, next) : ptr * ptr * ptr)
+    'l [] [lseg prev first next ~> l] (l = nil)
+    '(_ : unit) tt [] (first = next)
+    elim_lseg_nil_spec) As elim_lseg_nil.
+  Proof.
+    init_lemma ((prev, first), next) l ->; unfold lseg; SL.normalize.
+    Intro ->; Apply; reflexivity.
+  Qed.
+
+  Derive intro_lseg_cons_spec SuchThat (
+    VLem SPEC ((pr, p0, p1, pn) : ptr * ptr * ptr * ptr)
+    '(hd, tl) [] [vcell vP p0 ~> hd; lseg p0 p1 pn ~> tl] (prev hd = pr /\ next hd = p1)
+    '(_ : unit) tt [lseg pr p0 pn ~> (existT _ p0 (data hd)) :: tl] True
+    intro_lseg_cons_spec) As intro_lseg_cons.
+  Proof.
+    init_lemma (((pr, p0), p1), pn) ([], tl) [<- <-].
+    unfold lseg; SL.normalize.
+    Intro <-.
+    Apply. auto.
+    reflexivity.
+  Qed.
+
+  Derive elim_lseg_cons_spec SuchThat (
+    VLem SPEC ((pr, p0, pn) : ptr * ptr * ptr)
+    'l [] [lseg pr p0 pn ~> l] (is_cons l)&REQ
+    '(p1 : ptr) hd [vcell vP p0 ~> {| data := hd; prev := pr; next := p1 |}; lseg p0 p1 pn ~> tl_tot l REQ]
+      (hd_tot l REQ = existT _ p0 hd)
+    elim_lseg_cons_spec) As elim_lseg_cons.
+  Proof.
+    init_lemma ((pr, p0), pn) [|[p0' hd] tl] [].
+    unfold lseg; cbn.
+    Intro ->.
+    Apply (lseg_first tl pn); Apply (hd, tt); SL.normalize.
+    Apply. auto.
+    reflexivity.
+  Qed.
+
+  Derive elim_lseg_nnull_spec SuchThat (
+    VLem SPEC ((pr, p0) : ptr * ptr)
+    'l [] [lseg pr p0 NULL ~> l] (p0 <> NULL)
+    '(p1 : ptr) (hd, tl) [vcell vP p0 ~> {| data := hd; prev := pr; next := p1 |}; lseg p0 p1 NULL ~> tl]
+       (l = existT _ p0 hd :: tl)
+    elim_lseg_nnull_spec) As elim_lseg_nnull.
+  Proof.
+    init_lemma (pr, p0) l NNULL.
+    unfold lseg; Intro <-.
+    destruct l as [|[p0' hd] tl]; cbn in *.
+      { exfalso; apply NNULL; reflexivity. }
+    Apply (lseg_first tl NULL); Apply (hd, (tl, tt)); SL.normalize.
+    Apply. auto.
+    reflexivity.
+  Qed.
+
+
+  Lemma lseg_sl_null_nil l pr pn
+    (N : lseg_first l pn = NULL):
+    SLprop.impp (lseg_sl pr l pn) (l = nil).
+  Proof.
+    destruct l as [|[]]; cbn.
+    - apply SLprop.impp_drop. reflexivity.
+    - cbn in N; subst.
+      eapply SLprop.impp_enough.
+      SLprop.split_impp; [apply vcell_non_null | apply SLprop.impp_True].
+      intuition congruence.
+  Qed.
+
+  Lemma lseg_null_nil pr p pn : impp_lemma (fun l => (
+    [lseg pr p pn ~> l], (p = NULL),
+    fun _ : unit => l = nil)).
+  Proof.
+    apply intro_impp_lemma; intros l ->.
+    unfold lseg; SL.normalize.
+    Intro N.
+    eapply SLprop.impp_enough. eapply lseg_sl_null_nil, N.
+    exists tt; tauto.
+  Qed.
+
+
+  Lemma lseg_first_app l0 l1 p2:
+    lseg_first (l0 ++ l1) p2 = lseg_first l0 (lseg_first l1 p2).
+  Proof.
+    case l0; reflexivity.
+  Qed.
+
+  Lemma lseg_sl_app l0 l1 pr pn:
+    SLprop.eq (lseg_sl pr (l0 ++ l1) pn) (lseg_sl pr l0 (lseg_first l1 pn)** lseg_sl (lseg_last pr l0) l1 pn).
+  Proof.
+    revert pr; induction l0 as [|[] l0 IH]; intro; cbn;
+      [|rewrite IH, lseg_first_app];
+      SL.normalize; reflexivity.
+  Qed.
+
+  Derive lseg_app_spec SuchThat (
+    VLem SPEC ((pr, pf0, pl0, pf1, pn) : ptr * ptr * ptr * ptr * ptr)
+    '(l0, l1) [] [lseg pr pf0 pf1 ~> l0; lseg pl0 pf1 pn ~> l1] (lseg_last pr l0 = pl0)
+    '(_ : unit) tt [lseg pr pf0 pn ~> (l0 ++ l1)] True
+    lseg_app_spec) As lseg_app.
+  Proof.
+    init_lemma ((((pr, pf0), pl0), pf1), pn) (l0, l1) <-.
+    unfold lseg; SL.normalize.
+    Intro [<- <-].
+    rewrite lseg_sl_app, lseg_first_app.
+    Apply; reflexivity.
+  Qed.
+End Lemmas.
+
+Section Impl.
+  Variables (CT : ConcreteProg.context) (iP : Param.impl vP CT).
+
+  Import VGroup.Tactics.
+  Hint Extern 1 (CTX.Trf.Tac.intro_rule _ (lseg ?prev ?p ?p ~> ?sl) _ _ _) =>
+    exact (lseg_nil_intro_rule prev p sl) : CtxTrfDB.
+
+
+  Definition lseg_case_res (p : ptr) (r : option ptr) : Vprop.p _ :=
+    vgroup match r with
+    | None    => []
+    | Some p1 => [vcell vP p~>; lseg p p1 NULL~>]
+    end.
+  Global Arguments lseg_case_res/.
+
+  Definition lseg_case_res_sel (pr : ptr) (p : ptr) (r : option ptr):
+      forall v : match r with None => unit | Some p1 => data_t vP p * lseg_t end,
+      Vprop.ty (lseg_case_res p r ~>) :=
+    match r with
+    | None    => fun     _    => tt
+    | Some p1 => fun '(x, tl) => ({| data := x; prev := pr; next := p1 |}, (tl, tt))
+    end.
+
+  Definition lseg_case_spec : FDecl SPEC
+    (p : ptr) & (pr : ptr) 'l [] [lseg pr p NULL ~> l] True
+    '(r : option ptr) v [lseg_case_res p r ~> lseg_case_res_sel pr p r v]
+      (match r as r return (if r then _ else _) -> Prop with
+       | None    => fun     _    => p =  NULL /\ l = nil
+       | Some p1 => fun '(x, tl) => p <> NULL /\ l = existT _ p x :: tl
+       end v).
+  Proof. Derived. Defined.
+
+  Definition lseg_case_impl : FragImpl lseg_case_spec CT := fun p pr =>
+    if Mem.ptr_eq p NULL
+    then
+      gLem (lseg_null_nil pr p NULL) tt;;
+      gLem elim_lseg_nil (pr, p, NULL);;
+      Ret None
+    else
+      'g_p1 <- gLem elim_lseg_nnull (pr, p);
+      'p1   <- read_next iP p;
+      gRewrite g_p1 p1;;
+      Ret (Some p1).
+  Lemma lseg_case : FragCorrect lseg_case_impl.
+  Proof.
+    solve_by_wlp.
+    - exists tt; auto.
+    - eexists (_, _); eauto.
+  Qed.
+
+
+  Definition Length_spec : FDecl SPEC
+    (p : ptr) & (pr : ptr)
+    'l [lseg pr p NULL ~> l] [] True
+    '(n : nat) tt [] (n = length l).
+  Proof. Derived. Defined.
+  Variable Length : Length_spec CT.
+
+  Definition Length_impl : FImpl Length := fun p0 pr =>
+    'r <- lseg_case p0 pr;
+    match r with
+    | None =>
+        gLem replace1 (lseg pr NULL NULL, lseg pr p0 NULL);;
+        Ret 0
+    | Some p1 =>
+        'n <- Length p1 p0;
+        gLem intro_lseg_cons (pr, p0, p1, NULL);;
+        Ret (S n)
+    end.
+  Lemma Length_correct : FCorrect Length_impl.
+  Proof. solve_by_wlp. Qed.
+
+End Impl.
+
+  Definition entries := [
+    f_entry Length_spec   Length_correct
+  ].
+End DLList.
