Test/DLList.v
@@ -1,0 +1,123 @@
+From SLFun     Require Import Util Values SL VProg.Main.
+From SLFun.Lib Require Malloc DLList.
+
+Import Util.List.
+Import SLNotations ListNotations VProg.Main.Notations FunProg.Notations.
+Import SL.Tactics.
+
+Module DL := SLFun.Lib.DLList.
+
+(* A test instantiation of the doubly linked list library *)
+
+Section Definitions.
+  Import DL.Param.
+
+  (* list cell *)
+
+  Definition lcell_t := DL.Param.lcell_t memdata.
+
+  Definition p_data (p : ptr) : ptr := p.
+  Definition p_prev (p : ptr) : ptr := S p.
+  Definition p_next (p : ptr) : ptr := S (S p).
+
+  Lemma lcell_p (p : ptr):
+    VRecord.p lcell_t [vptr (p_data p) ~>; vptr (p_prev p) ~>; vptr (p_next p) ~>]
+      (fun v => (data v, prev v, next v))
+      (fun dt pr nx => DL.Param.mk_lcell dt pr nx).
+  Proof.
+    constructor; cbn; reflexivity.
+  Qed.
+
+  Definition lcell (p : ptr) : Vprop.p lcell_t := VRecord.v (lcell_p p).
+  Global Arguments lcell : simpl never.
+
+  Definition lcell_unfold p sl:
+    CTX.Trf.Tac.unfold_rule (lcell p ~> sl) (VRecord.v (lcell_p p) ~> sl).
+  Proof.
+    reflexivity.
+  Qed.
+
+  Global Instance lcell_Struct : Malloc.Struct lcell 3.
+  Proof.
+    split; intro p.
+    do 2 rewrite
+        Malloc.split_free_range with (n := 1),
+        !Malloc.free_range_1,
+        PeanoNat.Nat.add_1_r
+      by (cbn; auto).
+    unfold Malloc.free_cell, lcell; SL.normalize.
+    apply SLprop.eq_iff_imp; split;
+      [ Intro v0; Intro v1; Intro v2; Apply (mk_lcell v0 v1 v2)
+      | Intro [v0 v1 v2]; Apply v0; Apply v1; Apply v2 ];
+      SL.normalize; reflexivity.
+  Qed.
+
+  Program Definition vP : DL.Param.vp := {| vcell := lcell |}.
+  Next Obligation.
+    unfold lcell; SL.normalize.
+    eapply SLprop.impp_enough.
+    SLprop.split_impp; [apply SLprop.cell_non_null | apply SLprop.impp_True..].
+    tauto.
+  Qed.
+
+End Definitions.
+
+Section Impl.
+  Variable CT : ConcreteProg.context.
+
+  Variables
+    (Init   : Malloc.Init_spec   CT)
+    (Malloc : Malloc.Malloc_spec CT)
+    (Length : DL.Length_spec vP  CT).
+
+  (* Set up automatic intro/elim of vprops *)
+
+  Local Hint Resolve lcell_unfold | 1 (CTX.Trf.Tac.unfold_rule (lcell ?p ~> ?sl) _) : CtxTrfDB.
+  (* NOTE: the default pattern does not work when interacting with definitions from [Lib.DLList],
+           probably because of a mismatch [lcell_t] versus [DL.Param.lcell_t memdata]. *)
+  Import VRecord.Tactics VGroup.Tactics.
+
+  (* implementations needed by the generic doubly linked list library *)
+  Definition iP : DL.Param.impl vP CT.
+  Proof.
+    refine {|
+      DL.Param.read_prev  := mkFrag (fun p       => Read (p_prev p));
+      DL.Param.write_prev := mkFrag (fun '(p, r) => Write (p_prev p) r);
+      DL.Param.read_next  := mkFrag (fun p       => Read (p_next p));
+      DL.Param.write_next := mkFrag (fun '(p, r) => Write (p_next p) r);
+    |}.
+    all:abstract solve_by_wlp.
+  Defined.
+
+  Definition Main_spec : FDecl SPEC
+    (_ : unit)
+    'u [] [Malloc.full_mem ~> u] True
+    '(r : nat) tt [vtrue ~> tt] (r = 1).
+  Proof. Derived. Defined.
+  Variable Main : Main_spec CT.
+
+  Definition Main_impl : FImpl Main := fun _ =>
+    Init tt;;
+    'p <- Malloc 3;
+    gLem (Malloc.make_struct lcell) p;;
+    Write (p_prev p) NULL;;
+    Write (p_next p) NULL;;
+    gLem (DL.intro_lseg_nil  vP) (p, NULL);;
+    gLem (DL.intro_lseg_cons vP) (NULL, p, NULL, NULL);;
+    'r <- Length p NULL;
+    gLem intro_true (vgroup [Malloc.malloc_env ~>; Malloc.allocated p ~>; DL.lseg vP NULL p NULL~>]);;
+    Ret r.
+  Lemma Main_correct : FCorrect Main_impl.
+  Proof.
+    solve_by_wlp.
+  Qed.
+
+End Impl.
+
+Definition entries := [
+  f_entry Main_spec     Main_correct
+] ++ Malloc.entries ++ DL.entries vP.
+
+Derive prog SuchThat (ConcreteProg.of_entries entries (aux := [existT _ _ iP]) prog)
+  As prog_correct.
+Proof. Derived. Qed.
